Rename FFibVars helpers and drop fold remnants

ChoiceType/theories/DenotationFibers.v
@@ -2,7 +2,6 @@
 
     Fiber modality helpers for ChoiceType denotations. *)
 
-From Stdlib Require Import Logic.FunctionalExtensionality Logic.PropExtensionality.
 From LocallyNameless Require Import Tactics.
 From ChoiceType Require Export Syntax.
 From ChoiceType Require Import BasicStore LocallyNamelessProps.
@@ -17,136 +16,42 @@ Notation "φ ⊫ ψ" :=
   (entails φ ψ)
   (at level 85, ψ at level 84, no associativity).
 
-Definition fib_vars_obligation_step
-    (x : atom)
-    (R : Store → WfWorld → Prop)
-    (ρ : Store) (m : WfWorld) : Prop :=
-  dom ρ ## {[x]} ∧
-  ∀ σ (Hproj : res_restrict m {[x]} σ),
-    R (ρ ∪ σ) (res_fiber_from_projection m {[x]} σ Hproj).
-
-Definition fib_vars_obligation
+Definition FFibVars_obligation
     (X : aset) (p : FQ) (ρ : Store) (m : WfWorld) : Prop :=
   dom ρ ## X ∧
   ∀ σ (Hproj : res_restrict m X σ),
     res_models_with_store (ρ ∪ σ)
       (res_fiber_from_projection m X σ Hproj) p.
 
-Lemma fib_vars_obligation_step_commute x y R ρ (m : WfWorld) :
-  x ≠ y →
-  x ∈ world_dom (m : World) →
-  y ∈ world_dom (m : World) →
-  fib_vars_obligation_step y (fib_vars_obligation_step x R) ρ m →
-  fib_vars_obligation_step x (fib_vars_obligation_step y R) ρ m.
-Proof.
-  intros Hxy Hxm Hym [Hρy Hy].
-  unfold fib_vars_obligation_step in *.
-  split.
-  - destruct (world_wf m) as [[σ Hσ] _].
-    set (σy := store_restrict σ {[y]}).
-    assert (Hprojy : res_restrict m {[y]} σy).
-    { exists σ. split; [exact Hσ | reflexivity]. }
-    destruct (Hy σy Hprojy) as [Hρσy_x _].
-    subst σy.
-    rewrite dom_union_L in Hρσy_x.
-    rewrite store_restrict_dom in Hρσy_x.
-    set_solver.
-  - intros σx Hprojx.
-    split.
-    + rewrite dom_union_L.
-      destruct Hprojx as [σ [Hσ Hσx]].
-      assert (Hdomσx : dom σx ⊆ {[x]}).
-      { rewrite <- Hσx, store_restrict_dom. set_solver. }
-      set_solver.
-    + intros σy Hprojy_after_x.
-      pose proof (res_projection_from_fiber_projection
-        m {[x]} {[y]} σx σy Hprojx Hprojy_after_x) as Hprojy.
-      assert (Hprojx_after_y :
-        res_restrict
-          (res_fiber_from_projection m {[y]} σy Hprojy) {[x]} σx).
-      {
-        assert (Hdomσx : dom σx = {[x]}).
-        {
-          destruct Hprojx as [σ0 [Hσ0 Hσ0x]].
-          rewrite <- Hσ0x, store_restrict_dom.
-          pose proof (wfworld_store_dom m σ0 Hσ0) as Hdomσ0.
-          set_solver.
-        }
-        destruct Hprojy_after_x as [σ [Hσfiber_x Hσy]].
-        destruct Hσfiber_x as [Hσm Hσx].
-        exists σ. split.
-        - apply res_fiber_from_projection_member; [exact Hσm | exact Hσy].
-        - rewrite <- Hdomσx. exact Hσx.
-      }
-      destruct (Hy σy Hprojy) as [_ Hyx].
-      specialize (Hyx σx Hprojx_after_y).
-      assert (Hfib_eq :
-        res_fiber_from_projection
-          (res_fiber_from_projection m {[y]} σy Hprojy) {[x]} σx Hprojx_after_y =
-        res_fiber_from_projection
-          (res_fiber_from_projection m {[x]} σx Hprojx) {[y]} σy Hprojy_after_x).
-      {
-        apply wfworld_ext. apply world_ext.
-        - reflexivity.
-        - intros τ. simpl. tauto.
-      }
-      replace (ρ ∪ σx ∪ σy) with (ρ ∪ σy ∪ σx).
-      2:{
-        assert (Hdomσx : dom σx = {[x]}).
-        {
-          destruct Hprojx as [σ0 [Hσ0 Hσ0x]].
-          rewrite <- Hσ0x, store_restrict_dom.
-          pose proof (wfworld_store_dom m σ0 Hσ0) as Hdomσ0.
-          set_solver.
-        }
-        assert (Hdomσy : dom σy = {[y]}).
-        {
-          destruct Hprojy as [σ0 [Hσ0 Hσ0y]].
-          rewrite <- Hσ0y, store_restrict_dom.
-          pose proof (wfworld_store_dom m σ0 Hσ0) as Hdomσ0.
-          set_solver.
-        }
-        assert (Hdisj_xy : σx ##ₘ σy).
-        {
-          apply map_disjoint_dom.
-          rewrite Hdomσx, Hdomσy. set_solver.
-        }
-        rewrite <- (assoc_L (∪) ρ σx σy).
-        rewrite <- (assoc_L (∪) ρ σy σx).
-        f_equal. symmetry. apply map_union_comm. exact Hdisj_xy.
-      }
-      rewrite <- Hfib_eq. exact Hyx.
-Qed.
-
-Lemma fib_vars_formula_fv_subset D (p : FQ) :
+Lemma FFibVars_formula_fv_subset D (p : FQ) :
   formula_fv (FFibVars D p) ⊆ lvars_fv D ∪ formula_fv p.
 Proof.
   simpl. set_solver.
 Qed.
 
-Lemma fib_vars_formula_fv D (p : FQ) :
+Lemma FFibVars_formula_fv D (p : FQ) :
   formula_fv (FFibVars D p) = lvars_fv D ∪ formula_fv p.
 Proof.
   simpl. reflexivity.
 Qed.
 
-Lemma fib_vars_models_elim D (p : FQ) ρ m :
+Lemma FFibVars_models_elim D (p : FQ) ρ m :
   res_models_with_store ρ m (FFibVars D p) →
-  fib_vars_obligation (lvars_fv D) p ρ m.
+  FFibVars_obligation (lvars_fv D) p ρ m.
 Proof.
-  unfold fib_vars_obligation.
+  unfold FFibVars_obligation.
   unfold res_models_with_store. simpl.
   intros Hm. destruct Hm as [_ [Hdisj Hfib]].
   split; [exact Hdisj |].
   intros σ Hproj. models_fuel_irrel (Hfib σ Hproj).
 Qed.
 
-Lemma fib_vars_models_intro D (p : FQ) ρ m :
+Lemma FFibVars_models_intro D (p : FQ) ρ m :
   formula_scoped_in_world ρ m (FFibVars D p) →
-  fib_vars_obligation (lvars_fv D) p ρ m →
+  FFibVars_obligation (lvars_fv D) p ρ m →
   res_models_with_store ρ m (FFibVars D p).
 Proof.
-  unfold fib_vars_obligation.
+  unfold FFibVars_obligation.
   intros Hscope [Hdisj Hfib].
   unfold res_models_with_store. simpl.
   split; [exact Hscope |].
